* some more stuff

LCF.v
@@ -1,13 +1,370 @@
 Require Export Basic.
 Require Export Common.
 Require Export MC.
+Require Import Sumbool.
+
+Notation "A '&&&' B" := (sumbool_and _ _ _ _ A B).
 
 Module Temp (P X V E B R:DecType) (Ev:Eval E X V V) (BEv:Eval B X V Bool).
 
 Module Import MCBase := MCBase P X V E B R Ev BEv.
 
+Fixpoint compatible (Defs:DefSet) (s:State) (tl:RichLabel) (C:Choreography) : Prop :=
+  (match C, tl with
+  | Call X,           R_Call Y p       => X = Y /\ In p (fst (Defs X))
+  | RT_Call X ps C',  R_Call Y p       => (X = Y /\ In p ps)
+                                          \/ (~In p ps /\ compatible Defs s tl C')
+  | RT_Call X ps C',  R_Com p _ q _    => disjoint (p::q::nil) ps /\ compatible Defs s tl C'
+  | RT_Call X ps C',  R_Sel p q _      => disjoint (p::q::nil) ps /\ compatible Defs s tl C'
+  | RT_Call X ps C',  R_Cond p         => ~In p ps /\ compatible Defs s tl C'
+  | Com p e q x;; C', R_Com p' v q' x' => (p=p' /\ q=q' /\ x=x' /\ v=eval_on_state e s p)
+                                          \/ (disjoint (p::q::nil) (p'::q'::nil) /\ compatible Defs s tl C')
+  | Com p _ q _;; C', R_Sel p' q' _    => (disjoint (p::q::nil) (p'::q'::nil) /\ compatible Defs s tl C')
+  | Com p _ q _;; C', R_Cond p'        => (~In p' (p::q::nil) /\ compatible Defs s tl C')
+  | Com p _ q _;; C', R_Call Y p'      => (~In p' (p::q::nil) /\ compatible Defs s tl C')
+  | Sel p q l;; C',   R_Sel p' q' l'   => (p=p' /\ q=q' /\ l=l')
+                                          \/ (disjoint (p::q::nil) (p'::q'::nil) /\ compatible Defs s tl C')
+  | Sel p q _;; C',   R_Com p' _ q' _  => (disjoint (p::q::nil) (p'::q'::nil) /\ compatible Defs s tl C')
+  | Sel p q _;; C',   R_Cond p'        => (~In p' (p::q::nil) /\ compatible Defs s tl C')
+  | Sel p q _;; C',   R_Call Y p'      => (~In p' (p::q::nil) /\ compatible Defs s tl C')
+  | Cond p e C1 C2,   R_Cond p'        => (p=p')
+                                          \/ (p<>p' /\ compatible Defs s tl C1 /\ compatible Defs s tl C2)
+  | Cond p _ C1 C2,   R_Com p' _ q' _  => (~In p (p'::q'::nil) /\ compatible Defs s tl C1 /\ compatible Defs s tl C2)
+  | Cond p _ C1 C2,   R_Sel p' q' _    => (~In p (p'::q'::nil) /\ compatible Defs s tl C1 /\ compatible Defs s tl C2)
+  | Cond p _ C1 C2,   R_Call Y p'      => (p<>p' /\ compatible Defs s tl C1 /\ compatible Defs s tl C2)
+  | _,                _                => False
+end)%MC.
 
+(*
+Fixpoint reduce_C (Defs:DefSet) (C:Choreography) (s:State) (tl:RichLabel) :=
+  (match C, tl with
+  | Call X,           R_Call Y p       => if (R.eq_dec X Y &&& In_dec P.eq_dec p (fst (Defs X)))
+                                            then (if (Nat.eq_dec (length (fst (Defs X))) 1)
+                                                  then snd (Defs X)
+                                                  else (RT_Call X (set_remove_pid p (fst (Defs X))) (snd (Defs X))))
+                                            else End
+  | RT_Call X ps C',  R_Call Y p       => if (R.eq_dec X Y &&& In_dec P.eq_dec p ps)
+                                          then (if (Nat.eq_dec (length ps) 1)
+                                                then C'
+                                                else (RT_Call X (set_remove_pid p ps) C'))
+                                          else End
+  | Com p e q x;; C', R_Com p' v q' x' => if (P.eq_dec p p' &&& P.eq_dec q q' &&& V.eq_dec (eval_on_state e s p) v)
+                                          then C'
+                                          else if disjoint_dec _ P.eq_dec (p::q::nil) (p'::q'::nil)
+                                               then reduce_C Defs C' s tl
+                                               else End
+  | Com p _ q _;; C', R_Sel p' q' _    => if (disjoint_dec _ P.eq_dec (p::q::nil) (p'::q'::nil))
+                                          then reduce_C Defs C' s tl
+                                          else End
+  | Com p _ q _;; C', R_Cond p'        => if (In_dec P.eq_dec p' (p::q::nil))
+                                          then End
+                                          else reduce_C Defs C' s tl
+  | Com p _ q _;; C', R_Call _ p'      => if (In_dec P.eq_dec p' (p::q::nil))
+                                          then End
+                                          else reduce_C Defs C' s tl
+  | Sel p q l;; C',   R_Sel p' q' l'   => if (P.eq_dec p p' &&& P.eq_dec q q' &&& eq_label_dec l l')
+                                          then C'
+                                          else if disjoint_dec _ P.eq_dec (p::q::nil) (p'::q'::nil)
+                                               then reduce_C Defs C' s tl
+                                               else End
+  | Sel p q _;; C',   R_Com p' _ q' _  => if (disjoint_dec _ P.eq_dec (p::q::nil) (p'::q'::nil))
+                                          then reduce_C Defs C' s tl
+                                          else End
+  | Sel p q _;; C',   R_Cond p'        => if (In_dec P.eq_dec p' (p::q::nil))
+                                          then End
+                                          else reduce_C Defs C' s tl
+  | Sel p q _;; C',   R_Call _ p'      => if (In_dec P.eq_dec p' (p::q::nil))
+                                          then End
+                                          else reduce_C Defs C' s tl
+  | Cond p b C1 C2,   R_Cond p'        => if P.eq_dec p p'
+                                          then if beval_on_state b s p
+                                               then C1 else C2
+                                          else If p ? b Then (reduce_C Defs C1 s tl) Else (reduce_C Defs C2 s tl)
+  | Cond p b C1 C2,   R_Com p' _ q' _  => if In_dec P.eq_dec p (p'::q'::nil)
+                                          then End
+                                          else If p ? b Then (reduce_C Defs C1 s tl) Else (reduce_C Defs C2 s tl)
+  | Cond p b C1 C2,   R_Sel p' q' _    => if In_dec P.eq_dec p (p'::q'::nil)
+                                          then End
+                                          else If p ? b Then (reduce_C Defs C1 s tl) Else (reduce_C Defs C2 s tl)
+  | Cond p b C1 C2,   R_Call _ p'      => if P.eq_dec p p'
+                                          then End
+                                          else If p ? b Then (reduce_C Defs C1 s tl) Else (reduce_C Defs C2 s tl)
+  | _, _ => End
+end)%MC.
+*)
 
+Fixpoint reduce_C (Defs:DefSet) (C:Choreography) (s:State) (tl:RichLabel) :=
+  (match C, tl with
+  | Call X,           R_Call _ p       => if Nat.eq_dec (set_size_pid (fst (Defs X))) 1
+                                          then snd (Defs X)
+                                          else RT_Call X (set_remove_pid p (fst (Defs X))) (snd (Defs X))
+  | RT_Call X ps C',  R_Call Y p       => if In_dec P.eq_dec p ps
+                                          then if Nat.eq_dec (set_size_pid ps) 1
+                                               then C'
+                                               else RT_Call X (set_remove_pid p ps) C'
+                                          else RT_Call X ps (reduce_C Defs C' s tl)
+  | RT_Call X ps C',  _                => RT_Call X ps (reduce_C Defs C' s tl)
+  | Com p e q x;; C', R_Com p' v q' x' => if (P.eq_dec p p' &&& P.eq_dec q q' &&& V.eq_dec (eval_on_state e s p) v)
+                                          then C'
+                                          else Com p e q x;; reduce_C Defs C' s tl
+  | Com p e q x;; C', _                => Com p e q x;; reduce_C Defs C' s tl
+  | Sel p q l;; C',   R_Sel p' q' l'   => if (P.eq_dec p p' &&& P.eq_dec q q' &&& eq_label_dec l l')
+                                          then C'
+                                          else Sel p q l;; reduce_C Defs C' s tl
+  | Sel p q l;; C',   _                => Sel p q l;; reduce_C Defs C' s tl
+  | Cond p b C1 C2,   R_Cond p'        => if P.eq_dec p p'
+                                          then if beval_on_state b s p
+                                               then C1 else C2
+                                          else If p ? b Then (reduce_C Defs C1 s tl) Else (reduce_C Defs C2 s tl)
+  | Cond p b C1 C2,   _                => If p ? b Then (reduce_C Defs C1 s tl) Else (reduce_C Defs C2 s tl)
+  | _, _ => End
+  end)%MC.
+
+Definition reduce_S (s:State) (tl:RichLabel) :=
+  match tl with
+  | R_Com _ v q x => update s q x v
+  | _             => s
+  end.
+
+Lemma reduce_sound : forall Defs C s tl, MCP_WF (Build_Program Defs C) ->
+  compatible Defs s tl C -> MCC_To Defs C s tl (reduce_C Defs C s tl) (reduce_S s tl).
+Proof.
+induction C; intros; induction tl; try inversion H0; simpl.
+- rewrite <- H1. elim Nat.eq_dec; intros.
+  + apply C_Call_Local'; auto.
+  + apply C_Call_Start'; auto.
+    elim (not_eq _ _ b); intros; auto.
+    inversion H3. 2: inversion H5.
+    elim (MCP_WF_Vars _ H r); auto.
+    red; simpl; auto. unfold Vars; simpl. eapply set_size_0; eauto.
+- apply C_Delay_Call; auto.
+    2: { apply IHC; auto. eapply MCP_WF_Call; eauto. }
+    clear H2 H0 H s IHC C r Defs.
+    induction l; simpl; auto.
+    split. split; intro; eapply H1; simpl; eauto.
+    apply IHl; repeat intro. inversion_clear H.
+    apply (H1 a0); split; simpl; auto.
+- apply C_Delay_Call; auto.
+    2: { apply IHC; auto. eapply MCP_WF_Call; eauto. }
+    clear H2 H0 H s IHC C r Defs.
+    induction l; simpl; auto.
+    split. split; intro; eapply H1; simpl; eauto.
+    apply IHl; repeat intro. inversion_clear H.
+    apply (H1 a0); split; simpl; auto.
+- apply C_Delay_Call; auto.
+    2: { apply IHC; auto. eapply MCP_WF_Call; eauto. }
+    clear H2 H0 H s IHC C r Defs.
+    induction l; simpl; auto.
+    split. intro; eapply H1; simpl; eauto.
+    apply IHl; repeat intro. apply H1; simpl; auto.
+- inversion_clear H1. rewrite H2. elim in_dec; [elim Nat.eq_dec | idtac]; intros.
+  + apply C_Call_Finish'; auto.
+  + apply C_Call_Enter'; auto.
+    elim (not_eq _ _ b); intros; auto.
+    inversion H1. 2: inversion H5.
+    generalize (MCP_WF_Main _ H); simpl; intros.
+    inversion H4. inversion H7.
+    apply set_size_0 in H5. elim H8; auto.
+  + elim b; auto.
+- inversion_clear H1. elim in_dec; intros.
+  + exfalso; auto.
+  + apply C_Delay_Call; auto.
+    2: { apply IHC; auto. eapply MCP_WF_Call; eauto. }
+    clear b H3 H0 H IHC.
+    induction l; simpl; auto.
+    simpl in H2. split; auto.
+- induction e.
+  + inversion H0. inversion_clear H1. inversion_clear H3. inversion_clear H4.
+    * rewrite H5, H2, H1, H3. clear H2 H1 H3 H5 H0.
+      elim P.eq_dec; intro Hp. 2: elim Hp; auto.
+      elim P.eq_dec; intro Hq. 2: elim Hq; auto.
+      elim V.eq_dec; intro Hv. 2: elim Hv; auto.
+      apply C_Com'.
+    * inversion_clear H1. red in H2.
+      elim P.eq_dec; intro Hp. elim (H2 p); rewrite Hp; simpl; auto.
+      elim P.eq_dec; intro Hq. elim (H2 q); rewrite Hq; simpl; auto.
+      elim V.eq_dec; intro Hv; simpl; apply C_Delay_Eta; auto.
+      ++ simpl. split; split; intro; auto; eapply H2; simpl; eauto.
+      ++ eapply IHC; auto. eapply MCP_WF_eta; eauto.
+      ++ simpl. split; split; intro; auto; eapply H2; simpl; eauto.
+      ++ eapply IHC; auto. eapply MCP_WF_eta; eauto.
+  + inversion_clear H0. apply C_Delay_Eta; auto.
+      ++ simpl. split; split; intro; auto; eapply H1; simpl; eauto.
+         split; right; left; eauto.
+      ++ eapply IHC; auto. eapply MCP_WF_eta; eauto.
+- induction e.
+  + inversion_clear H0. apply C_Delay_Eta; auto.
+      ++ simpl. split; split; intro; auto; eapply H1; simpl; eauto.
+         split; right; left; eauto.
+      ++ eapply IHC; auto. eapply MCP_WF_eta; eauto.
+  + inversion H0. inversion_clear H1. inversion_clear H3. inversion_clear H4.
+    * rewrite H2, H1. clear H2 H1.
+      elim P.eq_dec; intro Hp. 2: elim Hp; auto.
+      elim P.eq_dec; intro Hq. 2: elim Hq; auto.
+      elim eq_label_dec; intro Hl. 2: elim Hl; auto.
+      apply C_Sel'.
+    * inversion_clear H1. red in H2.
+      elim P.eq_dec; intro Hp. elim (H2 p); rewrite Hp; simpl; auto.
+      elim P.eq_dec; intro Hq. elim (H2 q); rewrite Hq; simpl; auto.
+      elim eq_label_dec; intro Hl; simpl; apply C_Delay_Eta; auto.
+      ++ simpl. split; split; intro; auto; eapply H2; simpl; eauto.
+      ++ eapply IHC; auto. eapply MCP_WF_eta; eauto.
+      ++ simpl. split; split; intro; auto; eapply H2; simpl; eauto.
+      ++ eapply IHC; auto. eapply MCP_WF_eta; eauto.
+- induction e.
+  + inversion H0. apply C_Delay_Eta.
+    * simpl. split; intro; auto; eapply H1; simpl; eauto.
+    * eapply IHC; auto. eapply MCP_WF_eta; eauto.
+  + inversion H0. apply C_Delay_Eta.
+    * simpl. split; intro; auto; eapply H1; simpl; eauto.
+    * eapply IHC; auto. eapply MCP_WF_eta; eauto.
+- induction e.
+  + inversion H0. apply C_Delay_Eta.
+    * simpl. split; intro; auto; eapply H1; simpl; eauto.
+    * eapply IHC; auto. eapply MCP_WF_eta; eauto.
+  + inversion H0. apply C_Delay_Eta.
+    * simpl. split; intro; auto; eapply H1; simpl; eauto.
+    * eapply IHC; auto. eapply MCP_WF_eta; eauto.
+- inversion_clear H2.
+  apply C_Delay_Cond.
+  + split; intro; eapply H1; simpl; eauto.
+  + eapply IHC1; auto. eapply MCP_WF_Then; eauto.
+  + eapply IHC2; auto. eapply MCP_WF_Else; eauto.
+- inversion_clear H2.
+  apply C_Delay_Cond.
+  + split; intro; eapply H1; simpl; eauto.
+  + eapply IHC1; auto. eapply MCP_WF_Then; eauto.
+  + eapply IHC2; auto. eapply MCP_WF_Else; eauto.
+- elim P.eq_dec; intro Hp. 2: elim Hp; auto.
+  case_eq (beval_on_state b s p); intro Hb; rewrite <- Hp.
+  + apply C_Then'; auto.
+  + apply C_Else'; auto.
+- inversion_clear H1. inversion_clear H3.
+  elim P.eq_dec; intro Hp. elim H2; auto.
+  apply C_Delay_Cond; auto.
+  + eapply IHC1; auto. eapply MCP_WF_Then; eauto.
+  + eapply IHC2; auto. eapply MCP_WF_Else; eauto.
+- inversion_clear H2.
+  apply C_Delay_Cond; auto.
+  + eapply IHC1; auto. eapply MCP_WF_Then; eauto.
+  + eapply IHC2; auto. eapply MCP_WF_Else; eauto.
+Qed.
+
+Lemma disjoint_Sel_Sel : forall p q l p' q' l',
+  disjoint_eta_rl (Sel p q l) (R_Sel p' q' l') -> disjoint (p::q::nil) (p'::q'::nil).
+Proof.
+intros. intro; intro. inversion_clear H.
+inversion_clear H1; inversion_clear H2.
+inversion_clear H0. inversion_clear H2; inversion_clear H5.
++ apply H. transitivity a; auto.
++ inversion_clear H2. 2: inversion H5.
+  apply H3. transitivity a; auto.
++ inversion_clear H0. 2: inversion H5.
+  apply H1. transitivity a; auto.
++ inversion_clear H0. 2: inversion H5.
+  inversion_clear H2. 2: inversion H0.
+  apply H4. transitivity a; auto.
+Qed.
+
+Lemma disjoint_Com_Com : forall p q e x p' q' v x',
+  disjoint_eta_rl (Com p e q x) (R_Com p' v q' x') -> disjoint (p::q::nil) (p'::q'::nil).
+Proof. intros. apply disjoint_Sel_Sel with left right; auto. Qed.
+
+Lemma disjoint_Com_Sel : forall p q e x p' q' l,
+  disjoint_eta_rl (Com p e q x) (R_Sel p' q' l) -> disjoint (p::q::nil) (p'::q'::nil).
+Proof. intros. apply disjoint_Sel_Sel with l left; auto. Qed.
+
+Lemma disjoint_Sel_Com : forall p q l p' v q' x,
+  disjoint_eta_rl (Sel p q l) (R_Com p' x q' v) -> disjoint (p::q::nil) (p'::q'::nil).
+Proof. intros. apply disjoint_Sel_Sel with l left; auto. Qed.
+
+Lemma disjoint_ps_Sel : forall p q l ps,
+  disjoint_ps_rl ps (R_Sel p q l) -> disjoint (p::q::nil) ps.
+Proof.
+intros. intro; intro. inversion_clear H0.
+induction ps; auto.
+inversion_clear H.
+inversion_clear H2; auto.
+rewrite H in H0. inversion_clear H0.
+inversion_clear H1; auto. inversion_clear H0; auto.
+Qed.
+
+Lemma disjoint_ps_Com : forall p v q x ps,
+  disjoint_ps_rl ps (R_Com p v q x) -> disjoint (p::q::nil) ps.
+Proof.
+intros. intro; intro. inversion_clear H0.
+induction ps; auto.
+inversion_clear H.
+inversion_clear H2; auto.
+rewrite H in H0. inversion_clear H0.
+inversion_clear H1; auto. inversion_clear H0; auto.
+Qed.
+
+Lemma disjoint_ps_Cond : forall p ps,
+  disjoint_ps_rl ps (R_Cond p) -> ~In p ps.
+Proof.
+induction ps; intros; simpl; auto.
+intro. inversion_clear H. simpl in H1.
+inversion_clear H0; auto.
+apply IHps; auto.
+Qed.
+
+Lemma disjoint_ps_Call : forall p ps X,
+  disjoint_ps_rl ps (R_Call X p) -> ~In p ps.
+Proof.
+induction ps; intros; simpl; auto.
+intro. inversion_clear H. simpl in H1.
+inversion_clear H0; auto.
+eapply IHps; eauto.
+Qed.
+
+Lemma reduce_compatible : forall Defs C s tl C' s',
+  MCC_To Defs C s tl C' s' -> compatible Defs s tl C.
+Proof.
+intros.
+induction H; simpl; auto.
++ induction eta; induction t; simpl; auto.
+  * right; split; auto.
+    apply disjoint_Com_Com in H; auto.
+  * split; auto. apply disjoint_Com_Sel in H; auto.
+  * split; auto. intro.
+    inversion_clear H. inversion_clear H1; auto.
+    inversion_clear H; auto.
+  * split; auto. intro.
+    inversion_clear H. inversion_clear H1; auto.
+    inversion_clear H; auto.
+  * split; auto. apply disjoint_Sel_Sel in H; auto.
+  * right; split; auto.
+    apply disjoint_Sel_Sel in H; auto.
+  * split; auto. intro.
+    inversion_clear H. inversion_clear H1; auto.
+    inversion_clear H; auto.
+  * split; auto. intro.
+    inversion_clear H. inversion_clear H1; auto.
+    inversion_clear H; auto.
++ induction t; simpl; auto.
+  * repeat split; auto. intro.
+    inversion_clear H. inversion_clear H2; auto.
+    inversion_clear H; auto.
+  * repeat split; auto. intro.
+    inversion_clear H. inversion_clear H2; auto.
+    inversion_clear H; auto.
++ induction t; simpl; auto.
+  * split; auto. apply disjoint_ps_Com in H; auto.
+  * split; auto. apply disjoint_ps_Sel in H; auto.
+  * split; auto. apply disjoint_ps_Cond; auto.
+  * apply disjoint_ps_Call in H; auto.
+Qed.
+
+Lemma reduce_unique_1 : forall Defs C s tl C' s',
+  MCP_WF (Build_Program Defs C) ->
+  MCC_To Defs C s tl C' s' -> C' = reduce_C Defs C s tl.
+Proof.
+intros.
+eapply MCC_To_deterministic_1; eauto.
+apply reduce_sound; auto.
+eapply reduce_compatible; eauto.
+Qed.
 
 Lemma diamond_Chor : forall Defs C s tl1 tl2 C1 C2 s1 s2,
   MCC_To Defs C s tl1 C1 s1 -> MCC_To Defs C s tl2 C2 s2 ->
@@ -171,8 +528,8 @@ rename Procedures0 into Defs, Main0 into C, b into s.
 intros.
 elim (chor_eq_dec C' C''); intro HC'C''; [left | right].
 + inversion H; inversion H0.
-  clear H H0 s'1 H16 C'1 H15 tl2 H10 s1 H12 C1 H11 Procs1 H9 s'0 H8.
-  clear C'0 H7 tl1 H2 s0 H4 C0 H3 Procs0 H1.
+  clear H H0 s'1 H16 C'1 H15 tl2 H10 s1 H12 C1 H11 Defs1 H9 s'0 H8.
+  clear C'0 H7 tl1 H2 s0 H4 C0 H3 Defs0 H1.
   revert H5 H13; rewrite <- H6, <- H14, <- HC'C''; clear H6 H14 HC'C'' Defs' Defs'' C''.
   intros HC HC'.
   split; auto.
@@ -201,17 +558,17 @@ rename Procedures1 into Defs', Main1 into C', s into s'.
 rename Procedures2 into Defs'', Main2 into C'', s0 into s''.
 rename Procedures0 into Defs, Main0 into C, b into s.
 intros.
-rewrite <- (MCP_To_Procs_stable _ _ _ _ _ _ _ H0);
-rewrite <- (MCP_To_Procs_stable _ _ _ _ _ _ _ H0) in H0.
-rewrite <- (MCP_ToStar_Procs_stable _ _ _ _ _ _ _ H);
-rewrite <- (MCP_ToStar_Procs_stable _ _ _ _ _ _ _ H) in H.
+rewrite <- (MCP_To_Defs_stable _ _ _ _ _ _ _ H0);
+rewrite <- (MCP_To_Defs_stable _ _ _ _ _ _ _ H0) in H0.
+rewrite <- (MCP_ToStar_Defs_stable _ _ _ _ _ _ _ H);
+rewrite <- (MCP_ToStar_Defs_stable _ _ _ _ _ _ _ H) in H.
 clear Defs' Defs''.
 revert C s tl2 C' s' C'' s'' H H0; induction tl1.
 + right.
   inversion H.
   rewrite <- H2, <- H4. eexists; split; eauto. constructor.
 + intros.
-
+Abort.
 
 
 
@@ -240,7 +597,7 @@ induction tl; simpl; intros.
       simpl in H0, H6; inversion H0; clear H0.
       rewrite <- H9 in H5, H; clear Main1 H9.
       rewrite <- H8 in H5, H; clear Procedures1 H8.
-      rewrite <- (MCP_To_Procs_stable _ _ _ _ _ _ _ H3) in H, H4, H5, H3.
+      rewrite <- (MCP_To_Defs_stable _ _ _ _ _ _ _ H3) in H, H4, H5, H3.
       clear Procedures0.
       rename Main0 into C', b into s', s0 into s''.
       induction c2.
@@ -258,14 +615,20 @@ induction tl; simpl; intros.
       inversion H4; simpl; auto.
       inversion H0. inversion H15.
     * inversion H3; inversion H.
-      clear H H3 t H12 s1 H14 C1 H13 Procs1 H11 a H6 s0 H8 C0 H7 Procs0 H0.
+      clear H H3 t H12 s1 H14 C1 H13 Defs1 H11 a H6 s0 H8 C0 H7 Defs0 H0.
       induction c3, c4. induction a, p.
       inversion H9; inversion H15. clear H9 H15.
       revert H4 H5 H10 H16.
       rewrite <- H0, <- H3, <- H6, <- H7, <- H8, H11.
       clear s'0 H11 Main1 H8 Procedures0 H0 Procedures1 H7 b H6 Main0 H3; intros.
       elim b; clear b; intros c' Hc'; inversion_clear Hc'.
+Abort.
+
+
+
+
 
 Lemma convergence : forall c tls1 tls2 c1 c2,
   c --[ tls1 ]-->* c1 -> c --[ tls2 ]-->* c2 ->
-  tls1 <> tls2 -> exists c', c1 --[ tl2 ]--> c' /\ c2 --[ tl1 ]--> c'.
+  tls1 <> tls2 -> exists c', c1 --[ tls2 ]-->* c' /\ c2 --[ tls1 ]-->* c'.
+
